Testing the speed of a more inefficient implementation of a trellis-like structure in order to work out whether I'm making the right decision by implementing the trellis in the way I'm currently implementing it. Motivated by desire to change my implementation of the trellis in order to make it easier to prove things.

convolutional_codesScript.sml
@@ -982,12 +982,12 @@ Datatype:
 End
 
 (* -------------------------------------------------------------------------- *)
-(* Viterbi trellis data                                                       *)
-(*                                                                            *)
-(* Function from time steps and states to number of errors on optimal path to *)
-(* this point in the trellis and previous state on optimal path to this point *)
-(* in the trellis                                                             *)
+(* Returns the portion of the input bitstring which is relevant to the        *)
+(* current time-step                                                          *)
 (* -------------------------------------------------------------------------- *)
+(*Definition relevant_input_def:
+  relevant_input m bs t = TAKE m.output_length (DROP ((t - 1) * m.output_length) bs)
+End*)
 
 (* -------------------------------------------------------------------------- *)
 (* Returns the total number of errors that would be present if we took a path *)
@@ -1054,6 +1054,10 @@ Definition viterbi_trellis_node_def:
        prev_state := SOME best_origin_local.origin; |>
 End
 
+(*Definition viterbi_trellis_node_slow:
+  viterbi_trellis_node_slow m bs s t =
+End*) 
+
 (* -------------------------------------------------------------------------- *)
 (* Evaluate the trellis row-by-row, to take advantage of the dynamic          *)
 (* programming nature of the algorithm and ensure it evaluates efficiently.   *)
@@ -1086,15 +1090,16 @@ Definition example_recursive_grid_row_def:
   let
     prior_grid_row = example_recursive_grid_row n
   in
-    MAP (λn. (if 0 < n then EL (n - 1) prior_grid_row else 0) + EL n prior_grid_row + (if n < 9 then EL (n + 1) prior_grid_row else 0)) (COUNT_LIST 10)
+    MAP (λm. (if 0 < m then EL (m - 1) prior_grid_row else 0) + EL m prior_grid_row + (if m < 9 then EL (m + 1) prior_grid_row else 0)) (COUNT_LIST 10)
 End
 
 (* -------------------------------------------------------------------------- *)
-(* Testing whether or not example_grid takes an exponential amount of time    *)
-(* to compute. It could theoretically take an exponential amount of time if   *)
-(* the previous row was substituted in multiple places, and expanded out      *)
-(* fully multiple times. Each subsequent row would double the amount of time  *)
-(* taken because it has to do the computation from the previous row twice.    *)
+(* Testing whether or not example_recursive_grid_row takes an exponential     *)
+(* amount of time to compute. It could theoretically take an exponential      *)
+(* amount of time if the previous row was substituted in multiple places, and *)
+(* expanded out fully multiple times. Each subsequent row would double the    *)
+(* amount of time taken because it has to do the computation from the         *)
+(* previous row twice.                                                        *)
 (*                                                                            *)
 (* 100: 0.681                                                                 *)
 (* 200: 2.311                                                                 *)
@@ -1105,8 +1110,36 @@ End
 (* 700: 26.521                                                                *)
 (* 800: 34.426                                                                *)
 (* -------------------------------------------------------------------------- *)
-(*Theorem example_grid_time_test:
-  example_grid 800 = ARB
+(*Theorem example_recursive_grid_row_time_test:
+  example_recursive_grid_row 100 = ARB
+Proof
+  EVAL_TAC
+QED*)
+
+(* -------------------------------------------------------------------------- *)
+(* A similar test as above, with a slightly different definition.             *)
+(* -------------------------------------------------------------------------- *)
+Definition example_recursive_grid_row2_def:
+  example_recursive_grid_row2 0 = REPLICATE 10 1 ∧
+  example_recursive_grid_row2 (SUC n) =
+  MAP (λm. (if 0 < m then EL (m - 1) (example_recursive_grid_row2 n) else 0) + EL m (example_recursive_grid_row2 n) + (if m < 9 then EL (m + 1) (example_recursive_grid_row2 n) else 0)) (COUNT_LIST 10)
+End
+
+Theorem example_recursive_grid_row_example_recursive_grid_row2:
+  ∀n. example_recursive_grid_row n = example_recursive_grid_row2 n
+Proof
+  Induct_on ‘n’ >> gvs[example_recursive_grid_row_def, example_recursive_grid_row2_def]
+QED
+
+(* -------------------------------------------------------------------------- *)
+(* This implementation is much slower, as expected.                           *)
+(*                                                                            *)
+(* 2: 0.201                                                                   *)
+(* 3: 5.443                                                                   *)
+(* 4: 145.7                                                                   *)
+(* -------------------------------------------------------------------------- *)
+(*Theorem example_recursive_grid_row_time_test:
+  example_recursive_grid_row2 4 = ARB
 Proof
   EVAL_TAC
 QED*)
@@ -2733,7 +2766,7 @@ QED
 (* -------------------------------------------------------------------------- *)
 (* The number of errors present if we encoded the input bs with the state     *)(* machine m and compared it to the expected output rs.                       *)
 (* -------------------------------------------------------------------------- *)
-Definition get_num_errors:
+Definition get_num_errors_def:
   get_num_errors m rs bs = hamming_distance rs (vd_encode m bs)
 End
 
@@ -2743,8 +2776,8 @@ End
 (* and the function for calculating the total number of errors                *)
 (* -------------------------------------------------------------------------- *)
 Theorem get_num_errors_step_get_num_errors:
-  ∀m rs ps bol.
-  get_num_errors_step m rs ps bol = get_num_errors m rs
+  ∀m rs s r.
+  get_num_errors_step m () (viterbi_trellis_row m bs t) r = N (get_num_errors m rs (vd_find_optimal_code m s.origin )) + 
 Proof
 QED
 
@@ -3005,3 +3038,4 @@ Proof
         
 QED
 val _ = export_theory();
+
